backends/lean/Aeneas/Std/Scalar/Ops/Rem.lean
@@ -3,6 +3,7 @@ import Aeneas.Std.Scalar.Misc
 import Aeneas.Std.Scalar.Elab
 import Aeneas.Tactic.Solver.ScalarTac
 import Mathlib.Data.BitVec
+import Aeneas.Std.Scalar.Ops.CheckedArith
 
 namespace Aeneas.Std
 
@@ -12,10 +13,10 @@ open Result Error Arith ScalarElab WP
 # Remainder: Definitions
 -/
 def UScalar.rem {ty : UScalarTy} (x y : UScalar ty) : Result (UScalar ty) :=
-  if y.val != 0 then ok ⟨ BitVec.umod x.bv y.bv ⟩ else fail divisionByZero
+  if y.val != 0 then ok (UScalar.ofBitVec ty (BitVec.umod (UScalar.toBitVec x) (UScalar.toBitVec y))) else fail divisionByZero
 
 def IScalar.rem {ty : IScalarTy} (x y : IScalar ty) : Result (IScalar ty) :=
-  if y.val != 0 then ok ⟨ BitVec.srem x.bv y.bv ⟩
+  if y.val != 0 then ok (IScalar.ofBitVec ty (BitVec.srem (IScalar.toBitVec x) (IScalar.toBitVec y)))
   else fail divisionByZero
 
 def UScalar.try_rem {ty : UScalarTy} (x y : UScalar ty) : Option (UScalar ty) :=
@@ -24,11 +25,11 @@ def UScalar.try_rem {ty : UScalarTy} (x y : UScalar ty) : Option (UScalar ty) :=
 def IScalar.try_rem {ty : IScalarTy} (x y : IScalar ty) : Option (IScalar ty) :=
   Option.ofResult (rem x y)
 
-instance {ty} : HMod (UScalar ty) (UScalar ty) (Result (UScalar ty)) where
-  hMod x y := UScalar.rem x y
+instance {ty} : HCheckedRem (UScalar ty) (UScalar ty) (Result (UScalar ty)) where
+  hCheckedRem x y := UScalar.rem x y
 
-instance {ty} : HMod (IScalar ty) (IScalar ty) (Result (IScalar ty)) where
-  hMod x y := IScalar.rem x y
+instance {ty} : HCheckedRem (IScalar ty) (IScalar ty) (Result (IScalar ty)) where
+  hCheckedRem x y := IScalar.rem x y
 
 /-!
 # Sanity Checks
@@ -74,27 +75,27 @@ Theorems with a specification which uses integers and bit-vectors
 
 /-- Generic theorem - shouldn't be used much -/
 theorem UScalar.rem_bv_spec {ty} (x : UScalar ty) {y : UScalar ty} (hzero : y.val ≠ 0) :
-  x % y ⦃ z => (↑z : Nat) = ↑x % ↑y ∧ z.bv = x.bv % y.bv ⦄ := by
-  conv => arg 1; simp [HMod.hMod]
+  x %? y ⦃ z => (↑z : Nat) = ↑x % ↑y ∧ z.bv = x.bv % y.bv ⦄ := by
+  conv => arg 1; simp [HCheckedRem.hCheckedRem]
   simp [hzero, rem]
   simp only [val]
   simp
 
 /-- Generic theorem - shouldn't be used much -/
 theorem IScalar.rem_bv_spec {ty} (x : IScalar ty) {y : IScalar ty} (hzero : y.val ≠ 0) :
-  x % y ⦃ z => (↑z : Int) = Int.tmod ↑x ↑y ∧ z.bv = BitVec.srem x.bv y.bv ⦄ := by
-  conv => arg 1; simp [HMod.hMod]
+  x %? y ⦃ z => (↑z : Int) = Int.tmod ↑x ↑y ∧ z.bv = BitVec.srem x.bv y.bv ⦄ := by
+  conv => arg 1; simp [HCheckedRem.hCheckedRem]
   simp only [spec_ok, rem, bne_iff_ne, ne_eq, hzero, not_false_eq_true, ↓reduceIte]
   simp only [val]
   simp only [BitVec.toInt_srem, bv_toInt_eq, and_true]
 
 
 uscalar theorem «%S».rem_bv_spec (x : «%S») {y : «%S»} (hnz : y.val ≠ 0) :
-  x % y ⦃ z => (↑z : Nat) = ↑x % ↑y ∧ z.bv = x.bv % y.bv ⦄ :=
+  x %? y ⦃ z => (↑z : Nat) = ↑x % ↑y ∧ z.bv = x.bv % y.bv ⦄ :=
   UScalar.rem_bv_spec x hnz
 
 iscalar theorem «%S».rem_bv_spec (x : «%S») {y : «%S»} (hnz : y.val ≠ 0) :
-  x % y ⦃ z => (↑z : Int) = Int.tmod ↑x ↑y ∧ z.bv = BitVec.srem x.bv y.bv ⦄ :=
+  x %? y ⦃ z => (↑z : Int) = Int.tmod ↑x ↑y ∧ z.bv = BitVec.srem x.bv y.bv ⦄ :=
   IScalar.rem_bv_spec x hnz
 
 /-!
@@ -103,7 +104,7 @@ Theorems with a specification which only uses integers
 
 /-- Generic theorem - shouldn't be used much -/
 theorem UScalar.rem_spec {ty} (x : UScalar ty) {y : UScalar ty} (hzero : y.val ≠ 0) :
-  x % y ⦃ z => (↑z : Nat) = ↑x % ↑y ⦄ := by
+  x %? y ⦃ z => (↑z : Nat) = ↑x % ↑y ⦄ := by
   apply spec_mono
   · apply rem_bv_spec x hzero
   · intros x' h
@@ -111,18 +112,18 @@ theorem UScalar.rem_spec {ty} (x : UScalar ty) {y : UScalar ty} (hzero : y.val �
 
 /-- Generic theorem - shouldn't be used much -/
 theorem IScalar.rem_spec {ty} (x : IScalar ty) {y : IScalar ty} (hzero : y.val ≠ 0) :
-  x % y ⦃ z => (↑z : Int) = Int.tmod ↑x ↑y ⦄ := by
+  x %? y ⦃ z => (↑z : Int) = Int.tmod ↑x ↑y ⦄ := by
   apply spec_mono
   · apply rem_bv_spec x hzero
   · intros x' h
     exact h.1
 
 uscalar @[step] theorem «%S».rem_spec (x : «%S») {y : «%S»} (hnz : y.val ≠ 0) :
-  x % y ⦃ z => (↑z : Nat) = ↑x % ↑y ⦄ :=
+  x %? y ⦃ z => (↑z : Nat) = ↑x % ↑y ⦄ :=
   UScalar.rem_spec x hnz
 
 iscalar @[step] theorem «%S».rem_spec (x : «%S») {y : «%S»} (hnz : y.val ≠ 0) :
-  x % y ⦃ z => (↑z : Int) = Int.tmod ↑x ↑y ⦄ :=
+  x %? y ⦃ z => (↑z : Int) = Int.tmod ↑x ↑y ⦄ :=
   IScalar.rem_spec x hnz
 
 end Aeneas.Std
