backends/lean/Aeneas/Tactic/Solver/ScalarTac/Lemmas.lean
@@ -545,10 +545,7 @@ grind_pattern [agrind_nla] mod_lt => x % y
    to use (it has to be expressed in terms of `x.bv.toNat`). -/
 @[simp, scalar_tac_simps, grind =, agrind =]
 theorem UScalar.sizeOf {ty} (x : UScalar ty) : sizeOf x = x.val + 3 := by
-  cases x; simp only [UScalar.mk.sizeOf_spec, BitVec.sizeOf, Fin.sizeOf, BitVec.val_toFin]
-  unfold UScalar.val
-  simp only
-  omega
+  cases ty <;> cases x <;> simp [UScalar.val, UScalar.toNat]
 
 /-!
 # Nat.testBit
